\input{setup.tex}

\documentclass{article}
\usepackage{amsmath,unicode-math,slashed,physics,geometry,xcolor,hyperref}

\geometry{paperwidth=30cm, paperheight=80cm, margin=2.54cm, showframe}
\unimathsetup{math-style=ISO, bold-style=ISO, mathrm=sym}
\hypersetup{colorlinks=true,urlcolor=MaterialIndigo}
\definecolor{MaterialIndigo}{HTML}{3F51B5}

\setmainfont{FiraGO}[BoldFont=* SemiBold]
\setmonofont{Iosevka}

\def\WIEGHT{Regular}
\setmathfont{FiraMath-\WIEGHT.otf}[Path=../release/fonts/, BoldFont=*]
% \setmathfont{XITS Math}
% \setmathfont{STIX Two Math}

\def\bm#1{\symbfit{#1}}

\def\ee{\symrm{e}}
\def\ii{\symrm{i}}
\def\pp{\symrm{\pi}}

\def\dD{\symrm{D}}

\def\BesselJ{\symrm{J}}
\def\EulerGamma{\symrm{\Gamma}}

% TODO: script letters are not available
\def\lagL{\symscr{L}}
\def\actS{\symscr{S}}
\def\maniM{\symscr{M}}

\def\hodge{\ast} % TODO: \star is not available
\def\trans{{\symrm{T}}}

\def\infint{\int_{-\infty}^{+\infty}}
\def\fhalf{\frac{1}{2}}

\begin{document}

\section{Ramanujan's Formulas}

Ramanujan--Sato series (\url{https://en.wikipedia.org/wiki/Ramanujan%E2%80%93Sato_series})
\begin{align}
  \frac{1}{\pp}
  &= \frac{2\sqrt2}{99^2} \sum_{k=0}^{\infty} \frac{(4k)!}{k!^4} \frac{26390k+1103}{396^{4k}} \\
  &= \frac{12}{(640320)^{3/2}} \sum_{k=0}^{\infty}
     \frac{(6k)! (545140134k+13591409)}{(3k)! (k!)^3 (-2625 3741 2640 7680 00)^k} \\
  &= \frac{\sqrt{n}}{3} \sum_{m=0}^{\infty} \qty\big[6v(k)m + \bar{G}(k_1,\,k)] \, b_m c^m (k).
\end{align}

Rogers--Ramanujan continued fraction
(\url{http://mathworld.wolfram.com/Rogers-RamanujanContinuedFraction.html})
\begin{equation}
  r = \cfrac{1}{1+\cfrac{\ee^{-2\pp}}{1+\cfrac{\ee^{-4\pp}}{1+\cdots}}}
    = \frac{\fourthroot{5}\sqrt{\phi}-\phi}{\ee^{-2\pp/5}} \approx 1.
\end{equation}

Ramanujan's Integral I (\url{http://mathworld.wolfram.com/RamanujansIntegral.html})
\begin{equation}
  \infint \frac{\BesselJ_{\mu+\xi}(x)}{x^{\mu+\xi}} \frac{\BesselJ_{\nu-\xi}(y)}{y^{\nu-\xi}}
          \ee^{\ii t\xi} \dd{\xi}
  = \qty[\frac{2\cos(\fhalf t)}{x^2\ee^{-\ii t/2}+y^2\ee^{\ii t/2}}]^{(\mu+\nu)/2}
    \cdot \BesselJ_{\mu+\nu} \sqrt{2\cos(\fhalf t)\qty(x^2\ee^{-\ii t/2}+y^2\ee^{\ii t/2})}
    \cdot \ee^{\ii t(\nu-\mu)/2}.
\end{equation}

Ramanujan's Integral II
\begin{align}
     \int_0^\infty \frac{\dd{x}}{(1+x^2)\,(1+r^2x^2)\,(1+r^4x^2)\cdots}
  &= \frac{\pp}{2\,(1+r+r^3+r^6+r^{10}+\cdots)}; \\[1ex]
     \int_0^\infty \frac{(1+arx)\,(1+ar^2x)\cdots}{(1+x^2)\,(1+r^2x^2)\,(1+r^4x^2)\cdots}
     x^{n-1} \dd{x}
  &= \frac{\pp}{\sin n\pp} \prod_{m=1}^\infty \frac{(1-r^{m-n})\,(1-ar^m)}{(1-r^m)\,(1-ar^{m-n})}.
\end{align}

Ramanujan log-trigonometric integrals
(\url{http://mathworld.wolfram.com/RamanujanLog-TrigonometricIntegrals.html})
\begin{equation}
  \int_0^{\frac{\pp}{2}}
    \frac{\sqrt{\fhalf \sqrt{\frac{\ln^2\cos\theta}{\theta^2+\ln^2\cos\theta}} + \fhalf}}%
         {\fourthroot{\theta^2 + \ln^2\cos\theta}} \dd{\theta}
  = \frac{\pp}{2\sqrt{\ln 2}}.
\end{equation}
Generalization:
\begin{align}
  R_n^- &= \frac{2}{\pp} \int_0^{\pp/2} \qty(\theta^2+\ln^2\cos\theta)^{-2^{-n-1}}
           \sqrt{\fhalf+\fhalf\sqrt{\fhalf+\cdots+\fhalf\sqrt{
                                    \frac{\ln^2\cos\theta}{\theta^2+\ln^2\cos\theta}}}} \dd{\theta}
         = (\ln 2)^{-2^{-n}}, \\[1.2ex]
  R_n^+ &= \frac{2}{\pp} \int_0^{\pp/2} \qty(\theta^2+\ln^2\cos\theta)^{2^{-n-1}}
           \sqrt{\fhalf+\fhalf\sqrt{\fhalf+\cdots+\fhalf\sqrt{
                                    \frac{\ln^2\cos\theta}{\theta^2+\ln^2\cos\theta}}}} \dd{\theta}
         = (\ln 2)^{2^{-n}}.
\end{align}

Ramanujan cos/cosh identity (\url{http://mathworld.wolfram.com/RamanujanCosCoshIdentity.html})
\begin{equation}
    \qty(1+2\sum_{n=1}^\infty \frac{\cos  n\theta}{\cosh n\pp})^{-2}
  + \qty(1+2\sum_{n=1}^\infty \frac{\cosh n\theta}{\cosh n\pp})^{-2}
  = \frac{2\EulerGamma^4\qty(\frac{3}{4})}{\pp}.
\end{equation}

See \url{https://www.zhihu.com/question/26292855/answer/266846441}.

\section{Lagrangian and action}

Electromagnetism
\begin{equation}
  \lagL(x) = j^\mu(x) A_\mu(x) - \frac{1}{4\mu_0} F_{\mu\nu}(x) F^{\mu\nu}(x).
\end{equation}

Electromagnetism using differential forms
\begin{equation}
  \actS[\bm{A}] = -\int_{\maniM} \qty(\fhalf\bm{F}\wedge\hodge\bm{F} + \bm{A}\wedge\hodge\bm{J}).
\end{equation}

Dirac Lagrangian
\begin{equation}
  \lagL = \ii\hbar c\bar{\psi}\slashed{\partial}\psi - mc^2\bar{\psi}\psi.
\end{equation}

Quantum electrodynamic (QED) Lagrangian
\begin{equation}
  \lagL_{\mathrm{QED}}
  = \ii\hbar c\bar{\psi}\slashed{\dD}\psi - mc^2\bar{\psi}\psi
  - \frac{1}{4\mu_0} F_{\mu\nu} F^{\mu\nu}.
\end{equation}

Quantum chromodynamic (QCD) Lagrangian
\begin{equation}
  \lagL_{\mathrm{QCD}}
  = \sum_n \qty(\ii\hbar c\bar{\psi}_n\slashed{\dD}\psi_n - mc^2\bar{\psi}_n\psi_n)
  - \frac{1}{4} G^\alpha{}_{\mu\nu} G_\alpha{}^{\mu\nu}.
\end{equation}

Standard Model Lagrangian
\begingroup
\def\L{{\symrm{L}}}
\def\R{{\symrm{R}}}
\def\hc{\mathrm{h.c.}}
\begin{align}
  \lagL_{\mathrm{SM}}
  = &{} - \frac{1}{4} B_{\mu\nu}B^{\mu\nu} - \frac{1}{8} \tr(\bm{W}_{\mu\nu}\bm{W}^{\mu\nu})
        - \frac{1}{2} \tr(\bm{G}_{\mu\nu}\bm{G}^{\mu\nu})
        \tag*{[$U(1)$, $SU(2)$ and $SU(3)$ gauge]} \\
    &{} + \qty(\bar{\nu}_\L,\,\bar{e}_\L) \, \tilde{\sigma}^\mu \ii \dD_\mu \mqty(\nu_\L \\ e_\L)
        + \bar{e}_\R \sigma^\mu \ii \dD_\mu e_\R + \bar{\nu}_\R \sigma^\mu \ii \dD_\mu \nu_\R + \hc
        \tag*{[lepton dynamical]} \\
    &{} - \frac{\sqrt{2}}{v} \,
          \underbrace{\qty[  \qty(\bar{\nu}_\L,\,\bar{e}_\L) \, \phi M^e e_\R
                           + \bar{e}_\R \bar{M}^e \bar{\phi} \, \mqty(\nu_\L \\ e_\L)]}%
            _{\text{electron, muon, tauon}}
     {} - \frac{\sqrt{2}}{v} \,
          \overbrace{\qty[  \qty(-\bar{e}_\L,\,\bar{\nu}_\L) \, \phi^* M^\nu \nu_\R
                          + \bar{\nu}_\R \bar{M}^\nu \phi^\trans \mqty(-e_\L \\ \nu_\L)]}%
            ^{\text{neutrino}}
        \tag*{[lepton mass]} \\
    &{} + \qty(\bar{u}_\L,\,\bar{d}_\L) \, \tilde{\sigma}^\mu \ii \dD_\mu \mqty(u_\L \\ d_\L)
        + \bar{u}_\R \sigma^\mu \ii \dD_\mu u_\R + \bar{d}_\R \sigma^\mu \ii \dD_\mu d_\R + \hc
        \tag*{[quark dynamical]} \\
    &{} - \frac{\sqrt{2}}{v} \,
          \underbrace{\qty[  \qty(\bar{u}_\L,\,\bar{d}_\L) \, \phi M^d d_\R
                           + \bar{d}_\R \bar{M}^d \bar{\phi} \, \mqty(u_\L \\ d_\L)]}%
            _{\text{down, strange, bottom}}
     {} - \frac{\sqrt{2}}{v} \,
          \overbrace{\qty[  \qty(-\bar{d}_\L,\,\bar{u}_\L) \, \phi^* M^u u_\R
                          + \bar{u}_\R \bar{M}^u \phi^\trans \mqty(-d_\L \\ u_\L)]}%
            ^{\text{up, charmed, top}}
        \tag*{[quark mass]} \\
    % &{} - \frac{\sqrt{2}}{v} \qty[  \qty(\bar{u}_\L,\,\bar{d}_\L) \, \phi M^d d_\R
    %                               + \bar{d}_\R \bar{M}^d \bar{\phi} \, \mqty(u_\L \\ d_\L)]
    %     - \frac{\sqrt{2}}{v} \qty[  \qty(-\bar{d}_\L,\,\bar{u}_\L) \, \phi^* M^u u_\R
    %                               + \bar{u}_\R \bar{M}^u \phi^\trans \mqty(-d_\L \\ u_\L)]
    %     \tag*{[quark mass]} \\
    &{} + \overline{\dD_\mu\phi} \, \dD^\mu\phi
        - \frac{m_H^2}{2v^2} \qty(\bar{\phi}\phi-\frac{v^2}{2})^2
        \tag*{[Higgs dynamical and mass]}.
\end{align}
\endgroup

See \url{https://en.wikipedia.org/wiki/Lagrangian_(field_theory)} and
\url{http://einstein-schrodinger.com/Standard_Model.pdf}.

\end{document}

% \def\ee{\mathrm{e}}
% \def\ii{\mathrm{i}}
% \def\bm{\symbf}
% \newcommand{\innerprod}[2]{\left\langle{#1}\middle\vert{#2}\right\rangle}
% \newcommand{\brakket}[3]{\left\langle{#1}\middle\vert{#2}\middle\vert{#3}\right\rangle}
% % \newcommand{\ket}[1]{\left\lvert{#1}\right\rangle}
% % \newcommand{\bra}[1]{\left\langle{#1}\right\rvert}
% % \newcommand{\ip}[2]{\left\langle{#1}\middle\vert{#2}\right\rangle}
% % \newcommand{\op}[2]{\left\lvert{#1}\middle\rangle\middle\langle{#2}\right\rvert}
% % \newcommand{\dd}{\,\mathrm{d}}
% % \newcommand{\norm}[1]{\left\lVert{#1}\right\rVert}

% \[ g^{mn} g_{mn} T^{i}_{jk} \]

% \[ x \to \infty + \infty - \infty \]

% \begin{align*}
%      \int_{-\infty}^\infty \ee^{-x^2} \dd{x}
%   &= \qty[\int_{-\infty}^\infty \ee^{-x^2} \dd{x} \, \int_{-\infty}^\infty \ee^{-y^2} \dd{y}]^{1/2} \\
%   &= \qty[\int_0^{2\pi} \int_0^\infty \ee^{-r^2} r \dd{r}\dd{\theta}]^{1/2} \\
%   &= \qty[\pi \int_0^\infty \ee^{-u} \dd{u}]^{1/2} \\
%   &= \sqrt{\pi}
% \end{align*}


% \begin{align*}
% \int_{0}^aJ_0\left[\frac{x_n^{(0)}}{a}r\right]J_0\left[\frac{x_m^{(0)}}{a}r\right]r\dd{r}=\frac{a^2}{2}J_1^2[x_n^{(0)}]\delta_m^n.\\
% \int_{0}^{\infty}\frac{\cos x-\ee^{-x}}{x}\dd{x}=0\\
% \end{align*}
% \[\oint_{\partial\Sigma}\vec E\cdot \dd{\vec{l}}=-\frac{1}{c}\frac{\dd}{\dd t}\iint_{\Sigma}\vec B \cdot \dd{\vec{S}};\]
% \[\partial_{[a}F_{\beta\gamma]}=0;\quad \partial_\alpha F^{\alpha\beta}=\mu_0J^\beta\]
% \[\left(\frac{-\hbar^2}{2m}\nabla^2+V\right)\Psi=i\hbar\dot{\Psi}\]
% \[\begin{split}
% \frac{1}{\mathcal{C}^2}&{}=\frac{\innerprod{g'}{g'}}{\mathcal{C}^2}=\sum_{\bm{k}}\sum_{\bm{k}'}\brakket{g}{c_{\bm{k}',\uparrow}^\dagger c_{\bm{k}',\downarrow} c_{\bm{k},\downarrow}^\dagger c_{\bm{k},\uparrow}}{g}=\sum_{\bm{k}}\brakket{g}{c_{\bm{k},\uparrow}^\dagger c_{\bm{k},\downarrow} c_{\bm{k},\downarrow}^\dagger c_{\bm{k},\uparrow}}{g}\\
% &{}=\sum_{\bm{k}}\brakket{g}{n_{\bm{k},\uparrow}\left(1-n_{\bm{k},\downarrow}\right)}{g}\\
% &{}=\sum_{\norm{\bm{k}}<k_F^\downarrow}\brakket{g}{0}{g}+\sum_{k_F^\downarrow<\norm{\bm{k}}<k_F^\uparrow}\brakket{g}{1}{g}+\sum_{\norm{\bm{k}}>k_F^\uparrow}\brakket{g}{0}{g}\\
% &{}=N_\uparrow-N_\downarrow
% \end{split}\]
% \[\left[ f,g \right]\equiv \sum_{\alpha =1}^{s}{\left( \frac{\partial f}{\partial {{q}_{\alpha }}}\frac{\partial g}{\partial {{p}_{\alpha }}}-\frac{\partial g}{\partial {{q}_{\alpha }}}\frac{\partial f}{\partial {{p}_{\alpha }}} \right)}=\sum\limits_{\alpha =1}^{s}{\begin{vmatrix}
% 	\partial_{{q}_{\alpha }} f & \partial_{{p}_{\alpha }} f  \\
% 	\partial_{{q}_{\alpha }} g & \partial_{{p}_{\alpha }} g  \\
% 	\end{vmatrix} }=\sum\limits_{\alpha =1}^{s}{\frac{\partial \left( f,g \right)}{\partial \left( {{q}_{\alpha }},{{p}_{\alpha }} \right)}}\]
% \[\begin{split}
% & \frac{{{\text{d}}^{2}}f}{\text{d}{{t}^{2}}}=\frac{\text{d}}{\text{d}t}\left[ f,H \right]=\left[ \left[ f,H \right],H \right]=\hat{H}\hat{H}f={{{\hat{H}}}^{2}}f \\ 
% & \vdots  \\ 
% & \frac{{{\text{d}}^{n}}f}{\text{d}{{t}^{n}}}=\underbrace{\left[ \left[ \left[ f,H \right],\cdots  \right],H \right]}_{n}={{{\hat{H}}}^{n}}f  \\
% \end{split}\]
% \[\tilde{U}(r,z)=E_0\dfrac{\omega_0}{\omega(z)}\exp\left[-r^2\left(\dfrac{1}{\omega^2(z)}+\dfrac{\ii k}{2R(z)}\right)-\ii k z+\ii \zeta(z)\right]\]
% \[\omega(z)=\omega_0\sqrt{1+\left(\dfrac{\lambda z}{\pi {\omega_0}^2}\right)^2};\quad R(z)=z\left[1+\left(\dfrac{\pi {\omega_0}^2}{\lambda z}\right)^2\right]\]
% \[\left( \begin{matrix}
% {mg}/{l}\;+k-m\omega _{1}^{2} & -k  \\
% -k & {mg}/{l}\;+k-m\omega _{1}^{2}  \\
% \end{matrix} \right)\left( \begin{matrix}
% {{a}_{11}}  \\
% {{a}_{21}}  \\
% \end{matrix} \right)=0\]
% \[V=\underbrace{{{V}_{0}}}_{=0}+\underbrace{\sum\limits_{\alpha =1}^{s}{{{\left( \frac{\partial V}{\partial {{q}_{\alpha }}} \right)}_{0}}{{q}_{\alpha }}}}_{=0}+\underbrace{\frac{1}{2}\sum\limits_{\alpha ,\beta =1}^{s}{{{\left( \frac{{{\partial }^{2}}V}{\partial {{q}_{\alpha }}\partial {{q}_{\beta }}} \right)}_{0}}{{q}_{\alpha }}{{q}_{\beta }}}}_{>0}+\cdots \]
% \[T=\frac{1}{2}\sum\limits_{i=1}^{n}{{{m}_{i}}{{{\dot{\bm r}}}_{i}}\cdot {{{\dot{\bm r}}}_{i}}}=\frac{1}{2}\sum\limits_{\alpha ,\beta =1}^{s}{\left[ \sum\limits_{i=1}^{n}{{{m}_{i}}{{\left( \frac{\partial {{\bm r}_{i}}}{\partial {{q}_{\alpha }}} \right)}_{0}}\cdot {{\left( \frac{\partial {{\bm r}_{i}}}{\partial {{q}_{\beta }}} \right)}_{0}}} \right]{{{\dot{q}}}_{\alpha }}{{{\dot{q}}}_{\beta }}}+\cdots \]
% \[\left( \begin{matrix}
% {{u}_{0}}  \\
% {{u}_{1}}  \\
% \vdots   \\
% {{u}_{N-1}}  \\
% \end{matrix} \right)=\sum\limits_{k>0}{\left[ \left( \begin{matrix}
% 	1  \\
% 	\cos ka  \\
% 	\vdots   \\
% 	\cos k\left( N-1 \right)a  \\
% 	\end{matrix} \right)\underbrace{{{C}_{k+}}\cos \left( {{\omega }_{k}}t+{{\varphi }_{k+}} \right)}_{\frac{2}{\sqrt{N}}{{q}_{k+}}}+\left( \begin{matrix}
% 	0  \\
% 	\sin ka  \\
% 	\vdots   \\
% 	\sin k\left( N-1 \right)a  \\
% 	\end{matrix} \right)\underbrace{{{C}_{k-}}\cos \left( {{\omega }_{k}}t+{{\varphi }_{k-}} \right)}_{\frac{2}{\sqrt{N}}{{q}_{k-}}} \right]}\]
% \[G(\vec{r},{\vec{r}}',\tau )=\int _{-\infty }^{\infty }\tilde{G}(\vec{r},{\vec{r}}',\omega )e^{-i \tau  \omega }d\omega=\int_{-\infty }^{\infty } \frac{e^{-i \tau  \omega } e^{i k |\vec{r}-{\vec{r}}'| }}{(2 \pi ) |\vec{r}-{\vec{r}}'| } \, d\omega=\frac{\delta  \left(\tau -\frac{R}{c}\right)}{|\vec{r}-{\vec{r}}'| }\]
% \[
% \begin{split}	
% \mathcal{F}^{-1}(\ket{j})
% &{}=\frac{1}{\sqrt{2^n}}\sum_{k=0}^{2^n-1}\exp\left(-2\uppi \ii \frac{jk}{2^n}\right)\ket{k}.\\
% &{}=\frac{1}{\sqrt{2^n}}\sum_{k_{n-1}=0}^1\cdots\sum_{k_{0}=0}^1\exp\left(-2\uppi \ii j\sum_{l=0}^{n-1}\frac{2^l k_l}{2^n}\right)\ket{k_{n-1}\cdots k_0}\\
% &{}=\frac{1}{\sqrt{2^n}}\sum_{k_{n-1}=0}^1\cdots\sum_{k_{0}=0}^1\bigotimes_{l=1}^n\left[\exp\left(-2\uppi \ii j\frac{k_{n-l}}{2^l}\right)\ket{k_{n-l}}\right]\\
% &{}=\frac{1}{\sqrt{2^n}}\bigotimes_{l=1}^n\left[\sum_{k_{n-l}=0}^1\exp\left(-2\uppi \ii j\frac{k_{n-l}}{2^l}\right)\ket{k_{n-l}}\right]\\
% &{}=\frac{1}{\sqrt{2^n}}\bigotimes_{l=1}^n\left[\ket{0}_{n-l}+\ee^{-2\uppi \ii j /2^l}\ket{1}_{n-l}\right]\\
% &{}=\frac{1}{\sqrt{2^n}}\bigotimes_{l=1}^n\left[\ket{0}_{n-l}+\ee^{-2\uppi \ii ({0.j_{l-1}\ldots j_0})}\ket{1}_{n-l}\right].
% \end{split}
% \]

% \newcommand{\lb}{\left(}
% \newcommand{\rb}{\right)}
% \newcommand{\ec}{\text{,}}
% \newcommand{\ed}{\text{.}}
% \newcommand{\bt}{\lb t\rb}
% \newcommand{\deltaup}{\updelta}
% \newcommand{\piup}{\uppi}
% \newcommand{\ndd}{\,\mathrm{d}}
% \subsection*{Problem 1}
% For convenience, first we set $t_i=0$, and in the end, we replace $t_f$ by $t_f-t_i$ and right answer is obtained.
% The classical path is \[x_c\lb t\rb=A \cos\omega t+B\sin \omega t\ec\]where $A$ and $B$ can be determined by plugging $\lb0,x_i\rb$ and $\lb t_f, x_f\rb$ into the equation. The result is
% \[x_c\lb t\rb=x_i \cos\omega t+\frac{x_f-x_i\cos\omega t_f}{\sin\omega t_f}\sin \omega t\ed\]
% We write $x\lb t\rb=x_c\lb t\rb+\deltaup x\bt$. Due to the fact that $\deltaup x$ should vanish at $t=0$ and $t=t_f$, $\deltaup x$ can be expanded as sine series: \[\deltaup x\bt=\sum_{n=1}^\infty a_n\sin\frac{n\piup t}{t_f}\ed\]
% Also, the functional integral can be rewritten as \[\int\mathcal{D}\left[x\bt\right]=c\int\prod_{n=1}^\infty \dd a_n\ed\]
% So, we have
% \[L=\frac{m}{2}\lb\dot{x}_c+\deltaup\dot{x}\rb^2-\frac{m\omega^2}{2}\lb x_c+\deltaup x\rb^2\ec\]
% \[\dot{x}\bt=-\omega x_i \sin\omega t +\omega \frac{x_f-x_i\cos\omega t_f}{\sin\omega t_f}\cos\omega t+\sum_{n=1}^\infty\frac{a_n n \piup}{t_f}\cos\frac{n \piup t}{t_f}\ec\]
% \[S=\int_0^{t_f} L\ndd t\ed\]
% Because $x_c$ is the classical path, $\deltaup S_\text{classical}=0$, so there can't be any the linear term in the expression of $S$, and we also have in mind that the sine and cosine series are orthogonal. So, we can write S as following:
% \[\begin{split}S&{}=\frac{m}{2}\int_0^{t_f}\left[\lb-\omega x_i\sin\omega t+\omega \frac{x_f-x_i\cos\omega t_f}{\sin\omega t_f}\cos\omega t\rb^2+\sum_{n=1}^\infty\lb\frac{a_n n \piup}{t_f}\rb^2\cos^2\frac{n \piup t}{t_f}\right]\ndd t\\%
% &\quad{}-\frac{m\omega^2}{2}\int_0^{t_f}\left[\lb x_i\cos\omega t+ \frac{x_f-x_i\cos\omega t_f}{\sin\omega t_f}\sin\omega t\rb^2+\sum_{n=1}^\infty {a_n}^2\sin^2\frac{n \piup t}{t_f}\right]\ndd t\\%
% &{}=\sum_{n=1}^\infty\int_0^{t_f}\left[\frac{m}{2}\lb\frac{a_n n \piup}{t_f}\rb^2\cos^2\frac{n \piup t}{t_f}-\frac{m\omega^2}{2}{a_n}^2\sin^2\frac{n \piup t}{t_f}\right]\ndd t\\%
% &\quad{}+\frac{m\omega^2}{2}\int_0^{t_f}\left[ {x_i}^2-\lb\frac{x_f-x_i\cos\omega t_f}{\sin\omega t_f}\rb^2\right]\lb\sin^2\omega t-\cos^2\omega t\rb\ndd t\\%
% &\quad{}-\frac{m\omega^2}{2}\int_0^{t_f}4 {x_i}\lb\frac{x_f-x_i\cos\omega t_f}{\sin\omega t_f}\rb\lb\sin\omega t\cos\omega t\rb\ndd t\ed\end{split}\]
% Using 
% \[\int_0^{t_f}\lb\sin^2\omega t-\cos^2\omega t\rb\ndd t=-\frac{\sin2\omega t_f}{2\omega}\ec\]
% \[\int_0^{t_f}\sin\omega t\cdot\cos\omega t\ndd t=\frac{\sin^2\omega t_f}{2\omega}\ec\]
% \[\int_0^{t_f}\sin^2\frac{n\piup t}{t_f} \ndd t=\int_0^{t_f}\cos^2\frac{n\piup t}{t_f} \ndd t=\frac{a_n n \piup}{t_f}\ec\]
% we get
% \[S=\sum_{n=1}^\infty\left[\frac{m}{2}\lb\frac{a_n n \piup}{t_f}\rb^2-\frac{m\omega^2}{2}{a_n}^2\right]\frac{t_f}{2}+\frac{m\omega}{2\sin\omega t_f}\left[\lb {x_i}^2+{x_f}^2\rb\cos\omega t_f-2 x_i x_f\right]\ed\]
% \[\begin{split}U={}&\exp\left\{\frac{\ii}{\hbar}\frac{m\omega}{2\sin\omega t_f}\left[\lb {x_i}^2+{x_f}^2\rb\cos\omega t_f-2 x_i x_f\right]\right\}\\%
% &{}\times c\prod_{n=1}^{\infty}\int_{-\infty}^\infty\exp{\frac{\ii}{\hbar}\left[\frac{m}{2}\lb\frac{n \piup}{t_f}\rb^2-\frac{m\omega^2}{2}\right]\frac{t_f {a_n}^2}{2}}\ndd a_n\ed\end{split}\]
% Using the Fresnel integral formula:
% \[\int_{-\infty}^\infty\exp\lb \ii t\rb\ndd t=\sqrt{\piup \ii}\ec\]
% \[\int_{-\infty}^\infty\exp{\frac{\ii}{\hbar}\left[\frac{m}{2}\lb\frac{n \piup}{t_f}\rb^2-\frac{m\omega^2}{2}\right]\frac{t_f {a_n}^2}{2}}\ndd a_n\sim\frac{\sqrt{t_f}}{n}\ec\]
% \[U\lb x_f,t_f;x_i,t_i\rb=c'\lb t_f-t_i\rb\exp\left\{\frac{\ii m\omega}{2\hbar\sin\left[\omega \lb t_f-t_i\rb\right]}\left[\lb {x_i}^2+{x_f}^2\rb\cos\left[\omega\lb t_f-t_i\rb\right]-2 x_i x_f\right]\right\}\ed\]
% Because \[\int\dd x U\lb x_f,t_f;x,t\rb U\lb x,t;x_i,t_i\rb=U\lb x_f,t_f;x_i,t_i\rb\ec\]
% By using the Fresnel integral again:
% \[c'\lb t_f-t\rb c'\lb t-t_i\rb\sqrt{\frac{2 \piup \ii \hbar}{m \omega}\lb\frac{\cos\left[\omega\lb t_f-t\rb\right]}{\sin\left[\omega\lb t_f-t\rb\right]}+\frac{\cos\left[\omega\lb t-t_i\rb\right]}{\sin\left[\omega\lb t-t_i\rb\right]}\rb}=c'\lb t_f-t_i\rb\ec\]
% \[c'\lb t_f-t_i\rb=\sqrt{\frac{m\omega}{2\piup \ii \hbar\sin\left[\omega\lb t_f-t_i\rb\right]}}\ed\]
% Thus
% \[\begin{split}U\lb x_f,t_f;x_i,t_i\rb=&\sqrt{\frac{m\omega}{2\piup \ii \hbar\sin\left[\omega\lb t_f-t_i\rb\right]}}\\&{}\times\exp\left\{\frac{\ii m\omega}{2\hbar\sin\left[\omega \lb t_f-t_i\rb\right]}\left[\lb {x_i}^2+{x_f}^2\rb\cos\left[\omega\lb t_f-t_i\rb\right]-2 x_i x_f\right]\right\}\ed\end{split}\]
